Solved review comments.

src/Bedrock/P256/modinv/u320_sub.v
@@ -1,6 +1,8 @@
 From Stdlib Require Import BinInt String List InitialRing.
-From bedrock2 Require Import BasicC64Semantics WeakestPrecondition ProgramLogic.
+From bedrock2 Require Import BasicC64Semantics WeakestPrecondition ProgramLogic NotationsCustomEntry ZnWords.
 Import ListNotations ProgramLogic.Coercions SeparationLogic Array Scalars.
+Require Import bedrock2Examples.full_sub.
+From coqutil Require Import Tactics.Tactics WithBaseName.
 Local Open Scope string_scope. Local Open Scope Z_scope.
 
 Local Notation eval := (fold_right (fun (a : word) (s : Z) => a + 2^64*s) 0).
@@ -8,8 +10,8 @@ Local Notation array := (array scalar (word.of_Z 8)).
 
 (** * Specification *)
 
-Local Instance spec_of_u320_sub : spec_of "u320_sub" := 
-    fnspec! "u320_sub" (p_x p_y p_r : word) / (x y r : list word) R ~> b,
+#[export] Instance spec_of_u320_sub : spec_of "u320_sub" := 
+    fnspec! "u320_sub" (p_r p_x p_y : word) / (x y r : list word) R ~> b,
     {
         requires t m := 
             m =* array p_x x ⋆ array p_y y ⋆ array p_r r ⋆ R /\
@@ -19,10 +21,8 @@ Local Instance spec_of_u320_sub : spec_of "u320_sub" :=
             length r = 5%nat /\ eval r - 2^320*b = eval x - eval y
     }.
 
-Require Import bedrock2.NotationsCustomEntry bedrock2Examples.full_sub.
-
 (** * Implementation *)
-Definition u320_sub := func! (p_x, p_y, p_r) ~> b {
+Definition u320_sub := func! (p_r, p_x, p_y) ~> b {
     b = $0;
     unpack! d0, b = br_full_sub(load(p_x) , load(p_y), b);
     unpack! d1, b = br_full_sub(load(p_x + $8), load(p_y + $8) , b);
@@ -37,22 +37,20 @@ Definition u320_sub := func! (p_x, p_y, p_r) ~> b {
     store(p_r + $8 + $8 + $8 + $8, d4)
 }.
 
-Import coqutil.Tactics.Tactics bedrock2.ZnWords.
+Local Existing Instance spec_of_full_sub.
 
 Local Ltac lists_into_elements := repeat match goal with
   | H : length ?l = ?n |- _ =>  constr_eq true ltac:(isnatcst n);
   let x := fresh l "0" in destruct l as [|x l]; inversion H; clear H end.
 
-Local Existing Instance spec_of_full_sub.
 Lemma u320_sub_correct : program_logic_goal_for_function! u320_sub.
 Proof.
-    repeat straightline. lists_into_elements. unfold array in *.
+    repeat straightline. lists_into_elements. cbv [array] in *.
     repeat (straightline || straightline_call || ZnWords).
-    eexists [_ ; _ ; _ ; _ ; _]. intuition try ecancel_assumption. unfold fold_right. ZnWords.
+    eexists [_ ; _ ; _ ; _ ; _]. intuition try ecancel_assumption. cbn [fold_right]. ZnWords.
 Qed.
 
 (** * Linking Proof *)
-From coqutil Require Import WithBaseName.
 Definition u320_sub_funcs := &[, u320_sub; br_full_sub].
 
 Lemma link_full_sub : spec_of_u320_sub (Interface.map.of_list u320_sub_funcs).
